theories/examples_wp.v
@@ -10,10 +10,92 @@ Require Import base lang sugar free eval step wp wp_tactics encode notations.
 Context `{!osirisGS_gen hlc Σ}.
 
 
+(* ---------------------------------------------------------------------------*)
+(* Generated Examples (from a single file).
+   Only the formatting has been altered since generation, the definitions
+   themselves have not. *)
+
+
+
+(* Converting a single CMT file for [Test]. *)
+
+(* Auto generated headers. They import the required Coq modules:
+   - either translations of the dependencies of the present file
+   - or static dependencies defining the language
+   - or part of the verification of the [StdLib] (or maybe other verified libraries). *)
+(* TODO: get the From _ to work From libs *) Require Import Stdlib.
+
+
+(* Generated code: *)
+Definition a := (EInt 1).
+Definition b := (EInt 2).
+Definition c :=
+  (EApp (EApp (EMkPath ["Stdlib";"+"]) (EVar "a")) (EVar "b")).
+Definition truc :=
+  (EFun "x" (EFun "y"
+    (ELet (BiCons (Binding (PVar "t") (EVar "y")) BiNil)
+    (ELet (BiCons (Binding (PVar "z") (EVar "x")) BiNil)             
+    (EApp (EApp (EMkPath ["Stdlib";"+"]) (EVar "t")) (EVar "z")))))).
+Definition pleasedontclash (*This is not a name. *) :=
+   (EInt 0).
+
+
+
+(* Specification of the generated code.
+   (This part has not been generated.) *)
+Lemma a__spec s E:
+  ⊢ WP (eval EnvNil a) @s; E {{ λ v, ⌜v = VInt (int.repr 1)⌝ }}.
+Proof. by wp. Qed.
+
+Lemma b__spec s E:
+  ⊢ WP (eval EnvNil b) @s; E {{ λ v, ⌜v = VInt (int.repr 2)⌝ }}.
+Proof. by wp. Qed.
+
+Lemma c__spec s E:
+  let v1 := (VInt (int.repr 1)) in
+  let v2 := (VInt (int.repr 2)) in
+  let η :=
+    EnvCons "a" v1 $
+    EnvCons "b" v2 $
+    EnvCons "Stdlib" Stdlib $
+    EnvNil
+    in
+  ⊢ WP (eval η c) @s; E {{ λ v, ⌜v = VInt (int.repr 3)⌝ }}.
+Proof.
+  intros. wp.
+  wp_use Stdlib__add__spec; try done.
+  iIntros (v) "Hv". subst v1.
+  wp_use "Hv".
+Qed.
+
+(* [truc__spec] proves that [truc] indeed defines the addition. *)
+Lemma truc__spec s E:
+  let η :=
+    EnvCons "Stdlib" Stdlib $
+    EnvNil
+    in
+  ⊢ WP (eval η truc) @s; E
+       {{ λ add,
+            ∀ v1 i1,
+            ⌜v1 = VInt (int.repr i1)⌝ →
+            WP call add v1
+               {{ λ add1,
+                    ∀ v2 i2,
+                    ⌜v2 = VInt (int.repr i2)⌝ →
+                    WP call add1 v2
+                      {{ λ v, ⌜ v = VInt (int.repr (i1 + i2)) ⌝ }} }} }}.
+Proof.
+  iIntros. wp.
+  iIntros. wp_call.
+  iIntros. wp_call.
+  replace (i1 + i2)%Z with (i2 + i1)%Z; last lia.
+  by wp_use Stdlib__add__spec.
+Qed.
+
 
 
 (* ---------------------------------------------------------------------------*)
-(* Examples. *)
+(* Hand-Written Examples. *)
 
 
 (* let x = A() in y *)
