theories/libs/Stdlib.v
@@ -1,0 +1,36 @@
+From iris.proofmode Require Import base proofmode classes.
+From iris.base_logic.lib Require Import fancy_updates.
+From iris.bi Require Import weakestpre.
+From iris.prelude Require Import options.
+Import uPred.
+
+Require Import base lang sugar free eval step wp wp_tactics encode notations.
+
+Section StdLib.
+  Context `{!osirisGS_gen hlc Σ}.
+
+  Definition Stdlib__add : val :=
+    VClo EnvNil $
+      AnonFun "x" $
+      EFun "y" $
+      EIntAdd (EVar "x") (EVar "y").
+
+  Definition Stdlib :=
+    VStruct $
+      EnvCons "+" Stdlib__add EnvNil.
+
+  Lemma Stdlib__add__spec s E:
+    ∀ v1 v2 i1 i2,
+    v1 = VInt (int.repr i1) →
+    v2 = VInt (int.repr i2) →
+    ⊢ WP call Stdlib__add v1 @s; E
+         {{ λ v, WP call v v2 @s; E {{ λ v, ⌜v = VInt (int.repr (i1 + i2))⌝ }} }}.
+  Proof.
+    intros. subst. wp.
+    wp_call.
+    by rewrite int.add_repr_repr.
+  Qed.
+
+  Opaque Stdlib__add.
+End StdLib.
+
